Trying to add predicates on prophecies

erasure.v
@@ -4,34 +4,102 @@ From iris_io Require Export lang lang_erased.
 From iris.algebra Require Export ofe.
 From stdpp Require Import gmap.
 
+Record Proph_equiv  p p' :=
+  { PrA_eq : PrA p = PrA p';
+    PrP_eq :  match PrA_eq in _ = z return z → Stream expr with
+                eq_refl => PrP p end = PrP p' }.
+
+Lemma Proph_equiv_refl p : Proph_equiv p p.
+Proof.
+  unshelve econstructor; eauto.
+Qed.
+
 Definition have_same_proph
            (σ : language.state P_lang) (σ' : language.state PE_lang)
-  := σ.1 = σ'.1 ∧ dom (gset loc) σ.2 = σ'.2.
+  := σ.1 = σ'.1 ∧ dom (gset loc) σ.2 = dom (gset loc) σ'.2 ∧
+     ∀ x, x ∈ dom (gset loc) σ.2 →
+          ∃ v v', Proph_equiv v v' ∧
+                  σ.2 !! x = Some v ∧ σ'.2 !! x = Some v'.
 
-Definition conjure_prophecies (σ : language.state PE_lang) :
-  language.state P_lang :=
-  match σ with
-    (σh, σp) => (σh,  to_gmap (Sconst UnitV) σp)
-  end.
-
-Lemma conjure_prophecies_have_same_proph σ :
-  have_same_proph (conjure_prophecies σ) σ.
+Program Definition Proph_go_back p p'
+           (H : Proph_equiv p (Proph_tail p')) :=
+{|PrS := {|Shead := (Shead (PrS p')); Stail := PrS p |};
+  PrA := PrA p'; PrP := PrP p'; PrP_ent := PrP_ent p'; PrPvals := PrPvals p' |}.
+Next Obligation.
 Proof.
-  destruct σ; split; first done; simpl.
-  apply mapset.mapset_eq => x; split => Hx.
-  - destruct (decide (x ∈ m)); first done.
-    apply elem_of_dom in Hx. destruct Hx as [y Hy].
-    rewrite lookup_to_gmap option_guard_False //= in Hy.
-  - apply elem_of_dom. rewrite lookup_to_gmap option_guard_True; eauto.
+  intros p p' Pe.
+  destruct p as [pS pA pP pPv pP_ent pPSI].
+  destruct p' as [p'S p'A p'P p'Pv p'P_ent p'PSI].
+  simpl in *.
+  destruct Pe as [Pe1 Pe2]; simpl in *. destruct Pe1; subst.
+  destruct pPSI as [u Hu].
+  destruct (p'Pv u) as [y Hy].
+  destruct (p'P_ent 0 p'S y) as [x Hx]; auto.
+  rewrite Hy; exists u; done. simpl in *.
+  exists x. rewrite Hx; simpl.
+  destruct y as [yh yt]; simpl in *.
+  rewrite -Hy in Hu; simpl in *.
+  by apply proph_to_expr_inj in Hu; subst.
 Qed.
+
+Lemma Proph_tail_Proph_go_back p p' Heq :
+  Proph_tail (Proph_go_back p p' Heq) = p.
+Proof.
+  destruct p as [pS pA pP pPv pPe pPSI].
+  destruct p' as [p'S p'A p'P p'Pv p'Pe p'PSI].
+  destruct Heq as [Heq1 Heq2].
+  simpl in *.
+  destruct Heq1.
+  match goal with
+    |- ?A = ?B =>
+            eapply (Prohp_eq_simplify A B eq_refl)
+  end; auto.
+Qed.
+
+(* Lemma have_same_proph_refl σ : have_same_proph σ σ. *)
+(* Proof. *)
+(*   repeat split; auto. *)
+(*   intros x Hx. *)
+(*   apply elem_of_dom in Hx. destruct Hx as [y Hy]. *)
+(*   eexists _, _; repeat split; eauto. *)
+(* Qed. *)
+
+(* Hint Resolve have_same_proph_refl. *)
+
+(* Program Definition AllUnits := *)
+(* {| PrS := (Sconst UnitV); PrA := (); PrP := λ _, (Sconst Unit) |}. *)
+(* Next Obligation. *)
+(* Proof. *)
+(*   exists (). apply Seq_eq. *)
+(*   cofix IH. *)
+(*   rewrite [Sconst _]Stream_unfold [proph_to_expr _]Stream_unfold. *)
+(*   by apply Seq_refl. *)
+(* Qed. *)
+
+(* Definition conjure_prophecies (σ : language.state PE_lang) : *)
+(*   language.state P_lang := *)
+(*   match σ with *)
+(*     (σh, σp) => (σh, σp) *)
+(*   end. *)
+
+(* Lemma conjure_prophecies_have_same_proph σ : *)
+(*   have_same_proph (conjure_prophecies σ) σ. *)
+(* Proof. *)
+(*   destruct σ; split; first done; simpl. *)
+(*   apply mapset.mapset_eq => x; split => Hx. *)
+(*   - destruct (decide (x ∈ m)); first done. *)
+(*     apply elem_of_dom in Hx. destruct Hx as [y Hy]. *)
+(*     rewrite lookup_to_gmap option_guard_False //= in Hy. *)
+(*   - apply elem_of_dom. rewrite lookup_to_gmap option_guard_True; eauto. *)
+(* Qed. *)
 
 Lemma erased_reachable_reachable th1 h1 th2 σ2:
   rtc (@step PE_lang) (th1, (h1, ∅)) (th2, σ2) →
-  ∀ σ2', have_same_proph σ2' σ2 →
-         rtc (@step P_lang) (th1, (h1, ∅)) (th2, σ2').
+  ∀ σ2', have_same_proph σ2' σ2 → rtc (@step P_lang) (th1, (h1, ∅)) (th2, σ2').
 Proof.
   remember (th1, (h1, ∅)) as cfg.
   remember (th2, σ2) as cfg'.
+  rewrite {2}Heqcfg.
   intros Hrtc.
   revert th1 h1 th2 σ2 Heqcfg Heqcfg'.
   eapply (rtc_ind_r_weak (λ z z', ∀ (th1 : list (language.expr PE_lang)) (h1 : gmap loc val)
@@ -44,9 +112,9 @@ Proof.
                                rtc (@step P_lang) (th1, (h1, ∅)) (th2, σ2')));
   last eauto.
   - intros x th1 h1 th2 σ2 Heqcfg Heqcfg'; simplify_eq.
-    intros [σ2 σ2p] [Hh Hsp]; simpl in *.
-    rewrite Hh. rewrite (dom_empty_inv_L (D := gset loc) σ2p); last done.
-    econstructor.
+    intros [σ2 σ2p] [Hh [Hsp _]]; simpl in *.
+    rewrite dom_empty_L in Hsp. apply dom_empty_inv_L in Hsp. rewrite Hsp.
+    rewrite Hh.  econstructor.
   - intros x y z Hxy Hyz IH th1 h1 th2 σ2 Heqcfg Heqcfg' σ2' Hsp;
       simplify_eq; simpl in *.
     destruct y as [yh yp].
@@ -56,47 +124,86 @@ Proof.
       try (eapply rtc_r; first (by eapply IH; eauto); by repeat (econstructor; eauto)).
     all: destruct σ2' as [σ2'h σ2'p]; destruct Hsp as [Hsp1 Hsp2]; simpl in *; simplify_eq.
     + eapply (rtc_r _ (_ ++ fill K (Alloc _) :: _, (σ, σ2'p)));
-        [unshelve eapply (IH _ _ _ (_, _) _ _ (σ, σ2'p)); eauto; split; simpl; eauto|
+        [unshelve eapply (IH _ _ _ (_, σp) _ _ (σ, σ2'p)); eauto; split; simpl; eauto|
          repeat (econstructor; eauto)].
     + match goal with A : ?X.1 !! _ = _ |- _ => destruct X as [σmh σmp]; simpl in * end.
       eapply (rtc_r _ (_ ++ fill K (Load (Loc _)) :: _, (_, σ2'p)));
         [unshelve eapply (IH _ _ _ (σmh, σmp) _ _ (_, σ2'p)); eauto; split; simpl; eauto|
          repeat (econstructor; eauto)].
     + eapply (rtc_r _ (_ ++ fill K (Store (Loc _) _) :: _, (_, σ2'p)));
-        [unshelve eapply (IH _ _ _ (_, _) _ _ (_, σ2'p)); eauto; split; simpl; eauto|
+        [unshelve eapply (IH _ _ _ (_, σp) _ _ (_, σ2'p)); eauto; split; simpl; eauto|
          repeat (econstructor; eauto)].
     + match goal with A : ?X.1 !! _ = _ |- _ => destruct X as [σmh σmp]; simpl in * end.
       eapply (rtc_r _ (_ ++ fill K (CAS (Loc _) _ _) :: _, (_, σ2'p)));
-        [unshelve eapply (IH _ _ _ (_, _) _ _ (_, σ2'p)); eauto; split; simpl; eauto|
+        [unshelve eapply (IH _ _ _ (_, σmp) _ _ (_, σ2'p)); eauto; split; simpl; eauto|
          repeat (econstructor; eauto)].
     + eapply (rtc_r _ (_ ++ fill K (CAS (Loc _) _ _) :: _, (_, σ2'p)));
-        [unshelve eapply (IH _ _ _ (_, _) _ _ (_, σ2'p)); eauto; split; simpl; eauto|
+        [unshelve eapply (IH _ _ _ (_, σp) _ _ (_, σ2'p)); eauto; split; simpl; eauto|
          repeat (econstructor; eauto)].
-    + assert (({[fresh σp]} ∪ σp) ∖ {[fresh σp]} = σp) as Hfr.
-      { rewrite difference_union_distr_l_L difference_diag_L left_id_L.
-        apply difference_disjoint_L.
-        symmetry. apply disjoint_singleton_l, is_fresh. }
-      eapply (rtc_r _ (_ ++ fill K (Create_Pr) :: _, (_, delete (fresh σp) σ2'p)));
-        [unshelve eapply (IH _ _ _ (_, _) _ _ (_, _)); eauto; split; simpl; eauto|
+    + destruct Hsp2 as [Hsp21 Hsp22].
+      assert (dom (gset loc) (delete (fresh (dom (gset loc) σp)) σ2'p)
+                = dom (gset loc) σp) as Hfr.
+      { rewrite dom_delete_L Hsp21 dom_insert_L difference_union_distr_l_L
+                  difference_diag_L left_id_L difference_disjoint_L //=.
+          apply disjoint_singleton_r, is_fresh. }
+      eapply (rtc_r _ (_ ++ fill K (Create_Pr A P) :: _, (σ, delete (fresh (dom (gset loc) σp)) σ2'p)));
+        [unshelve eapply (IH _ _ _ (σ, σp) _ _ (_, _)); eauto; simpl; eauto|
          repeat (econstructor; eauto)].
-      * by rewrite (dom_delete_L (D := gset loc)) Hsp2 Hfr.
-      * destruct (elem_of_dom (D := gset loc) σ2'p (fresh σp)) as [[str Hstr]].
-        { rewrite Hsp2. by apply elem_of_union_l, elem_of_singleton. }
-        replace σ2'p with (<[fresh (dom (gset loc) (delete (fresh σp) σ2'p)) := str]> (delete (fresh σp) σ2'p)) at 2; last first.
-        { rewrite dom_delete_L Hsp2 Hfr insert_delete. by apply insert_id. }
-        rewrite -{2}Hfr -Hsp2 -dom_delete_L.
-        econstructor.
-    + assert (∃ str, σ2'p !! l = Some str) as [str Hstr]
-          by by apply (elem_of_dom (D := gset loc)).
+      * repeat split; auto; simpl.
+        intros x Hx. rewrite dom_delete_L in Hx.
+        apply elem_of_difference in Hx; destruct Hx as [Hx1 Hx2].
+        edestruct Hsp22 as (v1 & v2 & Hvv & Hv1 & Hv2); eauto.
+        apply not_elem_of_singleton in Hx2.
+        exists v1, v2; split; auto. split.
+        ++ rewrite lookup_delete_ne; auto.
+        ++ rewrite lookup_insert_ne in Hv2; auto.
+      * destruct (elem_of_dom (D := gset loc) σ2'p (fresh (dom (gset loc) σp))) as [[p Hp]].
+        { rewrite Hsp21 dom_insert.  by apply elem_of_union_l, elem_of_singleton. }
+        simpl.
+        replace σ2'p with (<[fresh (dom (gset loc) (delete (fresh (dom (gset loc) σp)) σ2'p)) := p]> (delete (fresh (dom (gset loc) σp)) σ2'p)) at 2; last first.
+        { rewrite Hfr. by rewrite insert_delete insert_id. }
+        rewrite -{2}Hfr.
+        destruct p as [str sA sP sSI].
+        destruct (Hsp22 (fresh (dom (gset loc) σp))) as (v1 & v2 & Hvv & Hv1 & Hv2); eauto.
+        rewrite lookup_insert in Hv2. rewrite Hp in Hv1.
+        inversion Hv1; inversion Hv2; simplify_eq.
+        destruct Hvv as [Hvv1 Hvv2]; simpl in *.
+        destruct Hvv1; simplify_eq.
+        apply Create_PrS.
+    + destruct Hsp2 as [Hsp21 Hsp22].
+      assert (∃ str, σ2'p !! l = Some str) as [str Hstr].
+      { apply (elem_of_dom (D := gset loc)).
+        rewrite Hsp21 dom_insert. by apply elem_of_union_l, elem_of_singleton. }
+      destruct (Hsp22 l) as (v1 & v2 & Hvv & Hv1 & Hv2); first apply elem_of_dom; eauto.
+      rewrite Hv1 in Hstr; inversion Hstr; subst; clear Hstr.
+      rewrite lookup_insert in Hv2; inversion Hv2; subst; clear Hv2.
       eapply (rtc_r _ (_ ++ fill K (Assign_Pr (Pr _) _) :: _,
-                       (_, <[l:={| Shead := v; Stail := str|}]> σ2'p)));
-        [unshelve eapply (IH _ _ _ (_, _) _ _ (_, _)); eauto; split; simpl; eauto|
+                       (_, <[l:= (Proph_go_back _ _ Hvv)]> σ2'p)));
+        [unshelve eapply (IH _ _ _ (_, σp) _ _ (_, _)); eauto; split; simpl; eauto|
          repeat (econstructor; eauto)].
-      * rewrite dom_insert_L. by apply subseteq_union_1_L, elem_of_subseteq_singleton.
-      * replace σ2'p with (<[l:= Stail {| Shead := v; Stail := str |}]>(<[l:={| Shead := v; Stail := str |}]> σ2'p)) at 2; last first.
-        { rewrite /= insert_insert. by apply insert_id. }
+      * assert (dom (gset loc) (<[l:=p]> σ2'p) = dom (gset loc) σ2'p) as Hσ2'p.
+        { rewrite dom_insert_L Hsp21 dom_insert_L assoc_L idemp_L.
+           rewrite subseteq_union_1_L //.
+           apply elem_of_subseteq_singleton, elem_of_dom; eauto. }
+        split; auto.
+        ++ rewrite dom_insert_L Hsp21 dom_insert_L assoc_L idemp_L.
+           rewrite subseteq_union_1_L //.
+           apply elem_of_subseteq_singleton, elem_of_dom; eauto.
+        ++ intros x. rewrite dom_insert_L. rewrite dom_insert_L in Hσ2'p.
+           rewrite Hσ2'p. intros Hx.
+           destruct (Hsp22 _ Hx) as (w1 & w2 & Hww & Hw1 & Hw2).
+           destruct (decide (x = l)); subst.
+           -- eexists (Proph_go_back str p Hvv), p; repeat split; auto;
+                last by rewrite lookup_insert.
+              unshelve econstructor; auto.
+           -- exists w1, w2; repeat split; auto; rewrite -?Hw2 lookup_insert_ne //.
+      * replace σ2'p with (<[l:= (Proph_tail (Proph_go_back str p Hvv))]>(<[l:= Proph_go_back str p Hvv]> σ2'p)) at 2; last first.
+        { apply map_eq => i. destruct (decide (i = l)); subst.
+          - rewrite lookup_insert Hv1. f_equal.
+            apply Proph_tail_Proph_go_back.
+          - do 2 rewrite lookup_insert_ne //=. }
         econstructor; auto.
-        rewrite lookup_insert //.
+        by rewrite lookup_insert.
 Qed.
 
 Definition safe e :=
@@ -109,15 +216,13 @@ Definition erased_safe e :=
     rtc (@step PE_lang) ([e], (∅, ∅)) (th2, σ2) →
     ∀ e, e ∈ th2 → AsVal e ∨ reducible e σ2.
 
-Lemma reducible_erase_reducible e σ σ' :
-  have_same_proph σ σ' →
-  reducible e σ →
-  @language.reducible PE_lang e σ'.
+Lemma reducible_erase_reducible e σ :
+  @language.reducible P_lang e σ →
+  @language.reducible PE_lang e σ.
 Proof.
-  intros Hsp (e'&σ2&efs&Hrd); simpl in *.
+  intros (e'&σ2&efs&Hrd); simpl in *.
   inversion Hrd as [K e1' e2' ? ? Hhrd]; simpl in *; subst.
-  destruct σ as [σh σp]; destruct σ' as [σ'h σ'p];
-    destruct Hsp as [? ?]; simpl in *; simplify_eq.
+  destruct σ as [σh σp]; simpl in *; simplify_eq.
   inversion Hhrd; subst; try (repeat econstructor; eauto; fail).
   + match goal with A : is_Some _ |- _ => destruct A as [? ?] end.
     repeat econstructor; eauto.
@@ -131,9 +236,9 @@ Lemma soundness_prophecies e :
   safe e → erased_safe e.
 Proof.
   intros Hs th2 σ2 Hrtc re Hre.
-  assert (rtc step ([e], (∅, ∅)) (th2, conjure_prophecies σ2)) as Hrtc'.
-  { eapply erased_reachable_reachable;
-      eauto using conjure_prophecies_have_same_proph. }
+  assert (rtc step ([e], (∅, ∅)) (th2, σ2)) as Hrtc'.
+  { eapply erased_reachable_reachable; eauto.
+    admit. }
   edestruct Hs as [?|Hred]; eauto.
   right. eapply reducible_erase_reducible;
            eauto using conjure_prophecies_have_same_proph.
