prelude/base.v
@@ -48,10 +48,34 @@ CoInductive Stream (A : Type) : Type :=
 Arguments Shead {_} _.
 Arguments Stail {_} _.
 
+Lemma Stream_unfold {A} (p : Stream A) : p = {|Shead := Shead p; Stail := Stail p|}.
+Proof. by destruct p. Qed.
+
 CoFixpoint Sconst {A : Type} (a : A) := {| Shead := a; Stail := Sconst a |}.
+
+CoInductive Seq {A : Type} : Stream A → Stream A → Prop :=
+  Seq_refl : forall x y t1 t2,
+    x = y → Seq t1 t2 → Seq {|Shead := x; Stail := t1|} {|Shead := y; Stail := t2|}.
+
+Lemma eq_Seq {A : Type} (x y : Stream A) : x = y → Seq x y.
+Proof.
+  intros ->; revert y.
+  cofix IH => y.
+  destruct y.
+  econstructor; auto.
+Qed.
+
+Axiom Seq_eq : ∀ {A : Type} (x y : Stream A), Seq x y → x = y.
 
 Fixpoint Snth {A : Type} n (s : Stream A) : A :=
   match n with
   | O => Shead s
   | S n' => Snth n' (Stail s)
+  end.
+
+Fixpoint take_nth_from {A : Type} n (s s' : Stream A) :=
+  match n with
+    O => {| Shead := Shead s; Stail := Stail s' |}
+  | S n' => {| Shead := Shead s';
+              Stail := take_nth_from n' (Stail s) (Stail s') |}
   end.
